proof/agp32_ID_CorrectScript.sml
@@ -1,0 +1,52 @@
+open hardwarePreamble translatorTheory translatorLib arithmeticTheory dep_rewrite blastLib bitstringSyntax fcpSyntax listSyntax wordsSyntax agp32StateTheory agp32EnvironmentTheory agp32ProcessorTheory ag32Theory ag32ExtraTheory ag32UtilitiesTheory agp32RelationTheory agp32UpdateTheory agp32InternalTheory agp32StepLib;
+
+(* correctness of ID stage items against the ISA *)
+val _ = new_theory "agp32_ID_Correct";
+
+val _ = prefer_num ();
+val _ = guess_lengths ();
+
+(** ID_PC **)
+Theorem agp32_Rel_ag32_ID_PC_correct:
+  !fext fbits a t I.
+    is_sch_decode I (agp32 fext fbits) ==>
+    Rel I (fext t) (agp32 fext fbits (t-1)) (agp32 fext fbits t) a t ==>
+    enable_stg 2 (agp32 fext fbits t) ==>
+    I (2,SUC t) <> NONE ==>
+    (agp32 fext fbits (SUC t)).ID.ID_PC = (FUNPOW Next (THE (I (2,SUC t)) − 1) a).PC
+Proof
+  rw [is_sch_decode_def] >>
+  Cases_on `I' (1,t) = NONE` >> fs [] >-
+   METIS_TAC [] >>
+  Q.ABBREV_TAC `s = agp32 fext fbits t` >>             
+  Q.ABBREV_TAC `s' = procs [agp32_next_state;WB_pipeline;MEM_pipeline;EX_pipeline;
+                            REG_write] (fext t) s s` >>
+  `(agp32 fext fbits (SUC t)).ID.ID_PC = (ID_pipeline (fext t) s s').ID.ID_PC`
+    by fs [agp32_ID_PC_updated_by_ID_pipeline,Abbr `s`,Abbr `s'`] >> rw [] >>
+  `s.ID.ID_ID_write_enable` by fs [enable_stg_def] >>
+  `s'.ID.ID_ID_write_enable`
+    by METIS_TAC [agp32_same_ID_items_before_ID_pipeline,Abbr `s`,Abbr `s'`] >>
+  rw [ID_pipeline_def] >>
+  fs [Rel_def,IF_Rel_def,IF_disable_Rel_def,Abbr `s`] >>
+  Cases_on `~enable_stg 1 (agp32 fext fbits (t − 1))` >> fs [] >>
+  Cases_on `reg_data_vaild 3 (agp32 fext fbits (t − 1))` >> fs [] >>
+  `(agp32 fext fbits (t-1)).MEM.MEM_state_flag`
+    by fs [enable_stg_def,agp32_IF_PC_write_enable_and_EX_MEM_flags] >>
+  fs [reg_data_vaild_def,enable_stg_def]
+QED
+
+(* ID stage *)
+Theorem agp32_Rel_ag32_ID_Rel_correct:
+  !fext fbits a t I.
+    is_sch_decode I (agp32 fext fbits) ==>
+    Rel I (fext t) (agp32 fext fbits (t-1)) (agp32 fext fbits t) a t ==>
+    enable_stg 2 (agp32 fext fbits t) ==>
+    I (2,SUC t) <> NONE ==>
+    ID_Rel (fext (SUC t)) (agp32 fext fbits (SUC t)) a (THE (I (2,SUC t)))
+Proof
+  rw [ID_Rel_def] >-
+   fs [agp32_Rel_ag32_ID_PC_correct] >>
+  cheat
+QED
+
+val _ = export_theory ();
